Use Adam Chlipala's WF recursion code

proofs/Vector.v
@@ -79,6 +79,21 @@ Fixpoint vec_length {A : Set} (tr : @vector A) : nat :=
                     end
   end.
 
+(* Source: http://adam.chlipala.net/cpdt/html/GeneralRec.html *)
+Definition vec_length_order {A : Set} (tr1 tr2 : @vector A) :=
+  vec_length tr1 < vec_length tr2.
+
+Hint Constructors Acc.
+
+Lemma vec_length_order_wf' :
+  forall len, forall A ls, vec_length ls <= len -> Acc (@vec_length_order A) ls.
+  unfold vec_length_order; induction len; crush.
+Defined.
+
+Theorem vec_length_order_wf {A : Set} : well_founded (@vec_length_order A).
+  red; intro; eapply vec_length_order_wf'; eauto.
+Defined.
+
 (*
 
 Definition vec_length {A : Set} (tr : @vector A) : nat :=
@@ -276,43 +291,58 @@ Fixpoint mkLeafAtHeight {A : Set} (ht : height) (v1 : A) : (vector) :=
 Definition join {A : Set} (a : @vector A) (b : @vector A) : (@vector A) :=
   Node (get_height a + 1) [ vec_length a ; (vec_length a + vec_length b) ] [a ; b].
 
+Inductive tmp_pair {A : Set} : Set :=
+| P : A -> (@vector A) -> tmp_pair.
 
-Program Fixpoint tryBottom_back {A : Set} (tr : @vector A) (v1 : A) {measure (vec_length tr)} : option (@vector A) :=
+
+Definition tryBottom_back {A : Set} (v1 : A) : (@vector A) -> option (@vector A).
+  refine (Fix vec_length_order_wf (fun _ => option (@vector A))
+  (fun (tr : @vector A)
+       (try_bottom_back : forall (tr' : @vector A), vec_length_order tr' tr -> option (@vector A)) =>
   match tr with
   | Leaf szs ns =>
     if length ns <? m
     then Some (Leaf (szs ++ [1]) (ns ++ [v1]))
     else None
   | Node ht szs trs =>
-    (match trs as trs' return trs = trs' -> option (vector) with
+    (match trs as trs' return trs = trs' -> option (@vector A) with
      | [] => fun _ => Some (Node ht [1] [mkLeafAtHeight (ht - 1) v1])
      | t :: ts  =>
        fun trs_not_nil =>
-         (match szs as szs' return szs = szs' -> option (vector) with
+         (match szs as szs' return szs = szs' -> option (@vector A) with
           | [] => fun _ => None
           | s :: ss =>
             fun szs_not_nil =>
-              let node_to_try := strong_last trs (cons_not_nil t ts) in
-              match tryBottom_back node_to_try v1 with
-              | Some has_v => let last_sz := strong_last szs (cons_not_nil s ss) in
-                              let szs' := removelast szs ++ [1 + last_sz] in
-                              let trs' := removelast trs ++ [has_v] in
-                              Some (Node ht szs' trs')
-              | None =>
-                if length trs <? m
-                then let branch  := mkLeafAtHeight (ht - 1) v1 in
-                     let last_sz := strong_last szs (cons_not_nil s ss) in
-                     let szs'    := szs ++ [1 + last_sz] in
-                     let trs'    := trs ++ [branch]
-                     in Some (Node ht szs' trs')
-                else None
+              let node_to_try := strong_last trs _ in
+              match try_bottom_back node_to_try _ with
+              | mb_vec => match mb_vec with
+                          | Some has_v => let last_sz := strong_last szs _ in
+                                          let szs' := removelast szs ++ [1 + last_sz] in
+                                          let trs' := removelast trs ++ [has_v] in
+                                          Some (Node ht szs' trs')
+                          | None =>
+                            if length trs <? m
+                            then let branch  := mkLeafAtHeight (ht - 1) v1 in
+                                 let last_sz := strong_last szs _ in
+                                 let szs'    := szs ++ [1 + last_sz] in
+                                 let trs'    := trs ++ [branch]
+                                 in Some (Node ht szs' trs')
+                            else None
+                          end
               end
           end) (eq_refl szs)
      end) (eq_refl trs)
-  end.
-  Admit Obligations.
+  end)).
+  Unshelve.
+  (* szs <> [] *)
+  + rewrite szs_not_nil. apply (cons_not_nil s ss).
+  + rewrite szs_not_nil. apply (cons_not_nil s ss).
+  (* trs <> [] *)
+  + rewrite trs_not_nil. apply (cons_not_nil t ts).
+  (* vec_length node_to_try < vec_length trs *)
+  + unfold vec_length_order. Admitted.
 
-Fixpoint tryBottom_front {A : Set} (tr : @vector A) (v1 : A) : option (@vector A) :=
+Fixpoint tryBottom_front {A : Set} (v1 : A) (tr : @vector A) : option (@vector A) :=
   match tr with
   | Leaf szs ns =>
     if length ns <? m
@@ -326,7 +356,7 @@ Fixpoint tryBottom_front {A : Set} (tr : @vector A) (v1 : A) : option (@vector A
        | [] => None
        | s :: ss =>
          let node_to_try := t in
-         match tryBottom_front node_to_try v1 with
+         match tryBottom_front v1 node_to_try with
          | Some has_v => let szs' := (1 + s) :: ss in
                          let trs' := has_v :: ts in
                          Some (Node ht szs' trs')
@@ -344,11 +374,11 @@ Fixpoint tryBottom_front {A : Set} (tr : @vector A) (v1 : A) : option (@vector A
 
 Definition insert {A : Set} (whr : wherE) (tr : vector) (v : A) : vector :=
   match whr with
-  | Front => match tryBottom_front tr v with
+  | Front => match tryBottom_front v tr with
              | Some has_v => has_v
              | None       => join (mkLeafAtHeight (get_height tr) v) tr
              end
-  | Back  => match tryBottom_back tr v with
+  | Back  => match tryBottom_back v tr with
              | Some has_v => has_v
              | None       => join tr (mkLeafAtHeight (get_height tr) v)
              end
