proofs/Examples.v
@@ -1,0 +1,84 @@
+Require Import Nat.
+Require Import List.
+Import ListNotations.
+
+From RRB Require Import Vector.
+
+(* -------------------------------------------------------------------------- *)
+
+Definition tree10 : vector :=
+  Node 1 [4 ; 8 ; 10]
+       [ Leaf [1 ; 1 ; 1 ; 1] [1 ; 2 ; 3 ; 4]
+       ; Leaf [1 ; 1 ; 1 ; 1] [5 ; 6 ; 7 ; 8]
+       ; Leaf [1 ; 1]         [9 ; 10]
+       ].
+
+Definition tree20 : vector :=
+  Node 2 [16 ; 20]
+         [ Node 1 [4 ; 8 ; 12 ; 16]
+                [ Leaf [1 ; 1 ; 1 ; 1] [1 ; 2 ; 3 ; 4]
+                ; Leaf [1 ; 1 ; 1 ; 1] [5 ; 6 ; 7 ; 8]
+                ; Leaf [1 ; 1 ; 1 ; 1] [9 ; 10 ; 11 ; 12]
+                ; Leaf [1 ; 1 ; 1 ; 1] [13 ; 14 ; 15 ; 16]
+                ]
+         ; Node 1 [4]
+                [ Leaf [1 ; 1 ; 1 ; 1] [17 ; 18 ; 19 ; 20]
+                ]
+       ].
+
+Definition tree_ub : vector :=
+  Node 2 [9 ; 21]
+         [ Node 1 [3 ; 6 ; 9]
+                [ Leaf [1 ; 1 ; 1] [1 ; 2 ; 3]
+                ; Leaf [1 ; 1 ; 1] [4 ; 5 ; 6]
+                ; Leaf [1 ; 1 ; 1] [7 ; 8 ; 9]
+                ]
+         ; Node 1 [3 ; 6 ; 10 ; 12]
+                [ Leaf [1 ; 1 ; 1]     [10 ; 11 ; 12]
+                ; Leaf [1 ; 1 ; 1]     [13 ; 14 ; 15]
+                ; Leaf [1 ; 1 ; 1 ; 1] [16 ; 17 ; 18 ; 19]
+                ; Leaf [1 ; 1]         [20 ; 21]
+                ]
+       ].
+
+Definition tree_ub2 : vector :=
+  Node 1 [1 ; 3 ; 6 ; 10]
+         [ Leaf [1]             [1]
+         ; Leaf [1 ; 1]         [2 ; 3]
+         ; Leaf [1 ; 1 ; 1]     [4 ; 5 ; 6]
+         ; Leaf [1 ; 1 ; 1 ; 1] [7 ; 8 ; 9 ; 10]
+         ].
+
+
+Definition tree_ub3 : vector :=
+  Node 1 [1 ; 2 ; 3 ; 4]
+       [ Leaf [1] [1]
+       ; Leaf [1] [2]
+       ; Leaf [1] [3]
+       ; Leaf [1] [4]
+       ].
+
+Definition tree17 : vector :=
+  Node 2 [16 ; 17]
+         [ Node 1 [4 ; 8 ; 10]
+                [ Leaf [1 ; 1 ; 1 ; 1] [1 ; 2 ; 3 ; 4]
+                ; Leaf [1 ; 1 ; 1 ; 1] [5 ; 6 ; 7 ; 8]
+                ; Leaf [1 ; 1 ; 1 ; 1] [9 ; 10 ; 11 ; 12]
+                ; Leaf [1 ; 1 ; 1 ; 1] [13 ; 14 ; 15 ; 16]
+                ]
+         ; Node 1 [1]
+                [ Leaf [1] [17] ]
+       ].
+
+Definition tree17_cons : vector :=
+  Node 2 [1 ; 17]
+         [ Node 1 [1] [ Leaf [1] [17] ]
+         ; Node 1 [4 ; 8 ; 12 ; 16]
+                  [ Leaf [1 ; 1 ; 1 ; 1] [1 ; 2 ; 3 ; 4]
+                  ; Leaf [1 ; 1 ; 1 ; 1] [5 ; 6 ; 7 ; 8]
+                  ; Leaf [1 ; 1 ; 1 ; 1] [9 ; 10 ; 11 ; 12]
+                  ; Leaf [1 ; 1 ; 1 ; 1] [13 ; 14 ; 15 ; 16]
+                  ]
+       ].
+
+Compute (toList (fromList (seq 1 17))).
